\documentclass[onecolumn]{article}
\usepackage{graphicx}
\usepackage{amsmath}
\usepackage{url}

\begin{document}
To show that the fully disordered free energy,
\begin{equation}
F_{fd}(T) = \frac{1}{\Omega}\sum_{i=1}^{\Omega}e_i  -  k_B T \ln(\Omega) ; ,
\end{equation}

is greater than or equal to the Helmholtz free energy, 
\begin{equation}
F(T) = -k_B T \ln(Z) = -k_B T \ln(Z) = -k_B T \ln(\sum_{i=1}^{\Omega} e^{-\frac{e_i}{k_BT}}) \;,
\end{equation}
it is sufficient to show that,
\begin{equation}
 f(N,T) - F(T) \geq 0. 
\end{equation}
Where $f(N,T)$ is the subspace kernel function given by, 
\begin{equation}
f(N,T) = \frac{1}{N}\sum_{i=1}^{N}e_i  -  k_B T \ln(N) \;,
\end{equation}
where $N\leq \Omega$.  
So the writing $f(N,T) - F(T) \geq 0$ explicitly gives,
\begin{equation}
\frac{1}{N}\sum_{i=1}^{N}e_i  +  k_B T [\ln(Z) -  \ln(N)] \geq 0  ;.
\end{equation}
Subtracting the  sum, dividing by $k_B T$ ,  then exponentiating, and then multiplying by $N$ gives, 
\begin{equation}
 Z = \sum_{i=1}^\Omega e^{-\frac{e_i}{k_B T}} \geq  N e^{-\frac{1}{k_B T N}\sum_{i=1}^{N}e_i} \;.
\end{equation}

With the set of energies is defined as begin ordered $\{e_i\}_{\Omega}\equiv e_1 \leq e_i \leq e_\Omega$ and the fact that all terms on the left side of the inequality are positive  it is sufficient to show that,
\begin{equation}
\sum_{i=1}^N e^{-\frac{e_i}{k_B T}} \geq  N e^{-\frac{1}{k_B T N}\sum_{i=1}^{N}e_i} \;,
\end{equation}
to prove that the subspace kernel function is greater than or equal to the exact Helmholtz free energy.  
Mathmaticaly this is equivalent to proving, 
\begin{equation}
\sum_{i=1}^N e^{-x_i} \geq  N e^{-\frac{1}{N}\sum_{i=1}^{N}x_i} \;.
\end{equation}
Where $x_i$ comes from a set of real numbers  $\{x_i\}_N$. 
\end{document}
